src/rocq/Handlers/MemoryModules/FiniteSizeof.v
@@ -178,33 +178,8 @@ End FinSizeof.
 Inductive UByte (uvalue : Type) :=
 | mkUByte (uv : uvalue) (dt : dtyp) (idx : N) (sid : store_id) : UByte uvalue.
 
-Module FinByte (LP:LLVMParams) : ByteImpl(LP)
-with  Definition SByte := UByte LP.DV.uvalue
-with  Definition uvalue_sbyte := mkUByte LP.DV.uvalue.
+Module FinByte (LP:LLVMParams) : ByteImpl(LP).
   Import LP.DV.
-
-  Definition SByte := UByte uvalue.
-
-  Definition uvalue_sbyte := mkUByte uvalue.
-
-  Definition sbyte_to_extractbyte (byte : SByte) : uvalue
-    := match byte with
-       | mkUByte uv dt idx sid => UVALUE_ExtractByte uv dt idx sid
-       end.
-
-  Lemma sbyte_to_extractbyte_inv :
-    forall (b : SByte),
-      {uv & {dt & {idx & {sid & sbyte_to_extractbyte b = UVALUE_ExtractByte uv dt idx sid}}}}.
-  Proof.
-    intros b. destruct b.
-    cbn; eauto.
-  Qed.
-
-  Lemma sbyte_to_extractbyte_of_uvalue_sbyte :
-    forall uv dt idx sid,
-      sbyte_to_extractbyte (uvalue_sbyte uv dt idx sid) =  UVALUE_ExtractByte uv dt idx sid.
-  Proof.
-    auto.
-  Qed.
-
+  Include ByteImpl LP.
+  
 End FinByte.
